New proof structure
Signed-off-by: zeramorphic <zeramorphic@proton.me>

ConNF/Counting/Recode.lean
@@ -93,20 +93,8 @@ theorem raisedSupportSet_small (S : Set (SupportCondition (top α))) (t : Tangle
 /-- A support for a `β`-tangle, expressed as a set of `α`-support conditions. -/
 def raisedSupport (S : Set (SupportCondition (top α))) (t : Tangle β) (hS : Small S) :
     OrdSupport (top α) :=
-  OrdSupport.strongSupport (raisedSupportSet S t) (raisedSupportSet_small S t hS)
-
-theorem raisedSupport_strong (S : Set (SupportCondition (top α))) (t : Tangle β)
-    (hS : Small S) (hS₁ : ∀ c ∈ S, Reduced c.value)
-    (hS₂ : ∀ c d, Reduced c.value → c <[α] d → d ∈ S → c ∈ S) :
-    (raisedSupport S t hS).Strong := by
-  refine OrdSupport.strongSupport_strong _ _ ?_ ?_
-  · rintro c (hc | hc)
-    · exact hS₁ c hc
-    · exact hc.2
-  · rintro c d hc hcd (hd | ⟨⟨e, he₁, he₂⟩, _⟩)
-    · exact Or.inl (hS₂ c d hc hcd hd)
-    · refine Or.inr ⟨?_, hc⟩
-      exact ⟨e, he₁, Relation.ReflTransGen.trans hcd.to_reflTransGen he₂⟩
+  sorry
+  -- OrdSupport.strongSupport (raisedSupportSet S t) (raisedSupportSet_small S t hS)
 
 /-- A set `s` of `β`-pretangles *appears* at level `α` if it occurs as the `β`-extension of some
 `α`-tangle. -/
@@ -219,18 +207,20 @@ theorem raisedSupport_supports (S : Set (SupportCondition (top α))) (t : Tangle
   refine congr_arg _ ?_
   refine (reducedSupport α t).supports _ ?_
   intro c hc
-  have := h (raise_reducedSupport_subset S t ⟨c, hc, rfl⟩)
-  rw [smul_raise_eq_iff] at this
-  exact this
+  sorry
+  -- have := h (raise_reducedSupport_subset S t ⟨c, hc, rfl⟩)
+  -- rw [smul_raise_eq_iff] at this
+  -- exact this
 
 theorem strongSupport_le_raisedSupport (β : Iio α) (t : Tangle (top α)) (u : Tangle β) :
     OrdSupport.strongSupport (reducedSupport α t) (reducedSupport α t).small ≤
     raisedSupport (reducedSupport α t) u (reducedSupport α t).small := by
-  constructor
-  · intro c hc
-    exact Or.inl hc
-  · intros
-    rfl
+  sorry
+  -- constructor
+  -- · intro c hc
+  --   exact Or.inl hc
+  -- · intros
+  --   rfl
 
 /-- Take the `β`-extension of `t`, treated as a set of `α`-level singletons, and turn them into
 coding functions. -/
@@ -238,21 +228,36 @@ def raiseSingletons (β : Iio α) (t : Tangle (top α)) : Set (CodingClass (top 
   (fun u => CodingClass.mk <| CodingFunction.code
     (raisedSupport (reducedSupport α t) u (reducedSupport α t).small)
     (singleton (top α) β (coe_lt_coe.mpr β.prop) u)
-    (raisedSupport_supports (reducedSupport α t) u _)) '' tangleExtension β t
+    (raisedSupport_supports (reducedSupport α t) u (reducedSupport α t).small)) ''
+      tangleExtension β t
 
--- TODO: Move next two lemmas.
+-- TODO: Change defn of `≤` to make this true.
+theorem equiv_of_le_equiv {β : Iic α} (S₁ S₂ T₁ T₂ : OrdSupport β)
+    (h₁ : S₁ ≤ T₁) (h₂ : S₂ ≤ T₂) (hT : T₁ ≈ T₂) : S₁ ≈ S₂ := by
+  sorry
 
-theorem reduced_of_mem_reducedSupport {β : Iic α} {t : Tangle β}
-    (c : SupportCondition β) (hc : c ∈ reducedSupport α t) :
-    Reduced c.value :=
-  hc.2
-
-theorem mem_reducedSupport_of_transConstrains_mem_reducedSupport {β : Iic α} {t : Tangle β}
-    (c d : SupportCondition β)
-    (hc : Reduced c.value) (hcd : c <[α] d) (hd : d ∈ reducedSupport α t) :
-    c ∈ reducedSupport α t := by
-  obtain ⟨e, he₁, he₂⟩ := hd.1
-  exact ⟨⟨e, he₁, Relation.ReflTransGen.trans hcd.to_reflTransGen he₂⟩, hc⟩
+theorem smul_reducedSupport_eq (β : Iio α) (t : Tangle (top α)) (V : OrdSupport (top α))
+    (hUV : OrdSupport.strongSupport (reducedSupport α t) (reducedSupport α t).small ≤ V)
+    (v : Tangle β) (ρ : Allowable (top α))
+    (hVW : ρ • raisedSupport (reducedSupport α t) v (reducedSupport α t).small ≈ V)
+    (c : SupportCondition (top α)) (hc : c ∈ (reducedSupport α t).carrier) : ρ • c = c := by
+  have := equiv_of_le_equiv
+    (OrdSupport.strongSupport (reducedSupport α t) (reducedSupport α t).small)
+    (ρ • OrdSupport.strongSupport (reducedSupport α t) (reducedSupport α t).small)
+    V
+    (ρ • raisedSupport (reducedSupport α t) v (reducedSupport α t).small)
+    hUV (OrdSupport.smul_le_smul (strongSupport_le_raisedSupport β t v) ρ) hVW.symm
+  have hc' := OrdSupport.cpos_smul_eq_cpos ρ this.symm c hc
+  have hS₁ := OrdSupport.smul_eq_of_smul_equiv ρ this.symm
+  have hS₂ := OrdSupport.strongSupport_strong (reducedSupport α t) (reducedSupport α t).small ?_ ?_
+  · simp_rw [OrdSupport.smul_cpos] at hc'
+    rw [hS₂.cpos_get_eq, hS₂.cpos_get_eq] at hc'
+    simp only [Allowable.smul_supportCondition, map_inv, Tree.inv_apply] at hc' ⊢
+    rw [← hc', smul_inv_smul]
+  · intro c hc
+    exact hc.2
+  · rintro c d hc hcd ⟨⟨e, he₁, he₂⟩, _⟩
+    exact ⟨⟨e, he₁, hcd.to_reflTransGen.trans he₂⟩, hc⟩
 
 theorem raiseSingletons_reducedSupport (β : Iio α) (t : Tangle (top α)) :
     {u | ∃ c ∈ raiseSingletons β t,
@@ -275,15 +280,10 @@ theorem raiseSingletons_reducedSupport (β : Iio α) (t : Tangle (top α)) :
     rw [Part.get_some, toPretangle_smul, Allowable.toStructPerm_smul, StructPerm.ofCoe_smul,
       singleton_toPretangle, smul_set_singleton, mem_singleton_iff] at hu
     subst hu
-    suffices : ρ • t = t
-    · rw [← mem_inv_smul_set_iff, Tree.comp_inv, ← StructPerm.ofCoe_smul, ← map_inv,
-        ← Allowable.toStructPerm_smul, ← toPretangle_smul (top α : IicBot α), ← this, inv_smul_smul]
-      exact hv
-    refine (reducedSupport α t).supports _ ?_
-    intro c hc
-    have := hUV.get_eq_get _ hc (hUV.mem_of_mem _ hc)
-    have := hVW.mem_left (hUV.mem_of_mem _ hc)
-    sorry
+    rw [← mem_inv_smul_set_iff, Tree.comp_inv, ← StructPerm.ofCoe_smul, ← map_inv,
+      ← Allowable.toStructPerm_smul, ← toPretangle_smul (top α : IicBot α),
+      ← (reducedSupport α t).supports _ (smul_reducedSupport_eq β t V hUV v ρ hVW), inv_smul_smul]
+    exact hv
   · simp only [ge_iff_le, mem_setOf_eq]
     intro hu
     obtain ⟨u, rfl⟩ := eq_toPretangle_of_mem (top α) β (coe_lt_coe.mpr β.prop) t u hu
@@ -307,6 +307,7 @@ theorem decodeRaised_raiseSingletons (β : Iio α) (t : Tangle (top α)) :
   intro u
   rw [decodeRaised_spec, raiseSingletons_reducedSupport]
 
+-- TODO: Quotient out by `o` to make it take an `OrdSupportOrbitClass` or something.
 noncomputable def raisedCodingFunction (β : Iio α) (cs : Set (CodingClass (top α)))
     (o : OrdSupportOrbit (top α)) (ho : ∀ U ∈ o, AppearsRaised β cs U)
     (ho' : ∀ U, ∀ hU : U ∈ o,
